\documentclass[10pt]{article}
\usepackage[utf8]{inputenc}
\usepackage[T1]{fontenc}
\usepackage{amsmath}
\usepackage{amsfonts}
\usepackage{amssymb}
\usepackage[version=4]{mhchem}
\usepackage{stmaryrd}
\usepackage{bbold}

\begin{document}
Moolels of TP. 1/10/24

Gaussian Inicgals\\
Let's consider the Gaussian distribution (PDF):

$$
p(x)=c e^{-\frac{a x^{2}}{2}} \quad a>0
$$

$p(x)$ must be nonneliged in $(-\infty,+\infty)$, so

$$
\int_{-\infty}^{+\infty} p(x) d x=1 \quad \Rightarrow \quad c \int_{-\infty}^{+\infty} e^{-\frac{a x^{2}}{2}} d x=1
$$

This gives the simplest form of Ganssion integral:\\
(1) $\quad \int_{-\infty}^{+\infty} e^{-\frac{a x^{2}}{2}} d x=\sqrt{\frac{2 \pi}{a}} \quad a>0$.

A viore general Gaussion integial:\\
(2) $\quad \int_{-\infty}^{+\infty} e^{-\frac{a x^{2}}{2}+b x} d x=$ ?

To solve it we use a change of vars.\\
Notice that the min. of the exponent has chagged.

$$
\frac{d}{d x}\left(-\frac{a x^{2}}{2}+b x\right)=-a x+b=0 \quad \Rightarrow \quad x=\frac{b}{a} \quad b \in \mathbb{R}
$$

We invioduce the new ver. $y=x-\frac{b}{a}$.

We subt this into the exponens:

$$
\begin{aligned}
&-\frac{a x^{2}}{2}+b x=-\frac{a}{2}\left(y+\frac{b}{a}\right)^{2}+b\left(y+\frac{b}{a}\right)=-\frac{a}{2}\left(y^{2}+\frac{2 b y}{a}+\left(\frac{b}{a}\right)^{2}\right)+b y+\frac{b^{2}}{a}= \\
&=-\frac{a}{2} y^{2}+\frac{b^{2}}{2 a} \\
& \int_{-\infty}^{+\infty} e^{-\frac{a x^{2}}{2}+b x} d x=\int_{-\infty}^{+\infty} e^{-\frac{a y^{2}}{2}+\frac{b^{2}}{2 a}} d y=e^{\frac{b^{2}}{2 a}} \int_{-\infty}^{+} e^{-\frac{a y^{2}}{2}} d y \Rightarrow
\end{aligned}
$$

(3) $\quad \int_{-\infty}^{+\infty} e^{-\frac{a x^{2}}{2}+b x} d x=\sqrt{\frac{2 \pi}{a}} e^{\frac{b^{2}}{2 a}} \quad a>0$

Left's colculate the infynal in $\varphi$. (3) when $b=i t, t \in \mathbb{R}$.

$$
\varphi(t)=\int_{-\infty}^{+\infty} d x e^{i x t} \sqrt{\frac{a}{2 \pi} e^{-\frac{a x^{2}}{2}}} \quad \text { 1) Fourier transf } \quad \text { of G.Pdf. } \quad \text { 2)ch.f. of G.pdf. } \quad .
$$

We take the time derivative of $\varphi$ :

$$
\varphi^{\prime}(t)=\sqrt{\frac{a}{2 \pi}} i \int d x \times e^{i x t} e^{-\frac{a}{2} x^{2}}
$$

why con we do this? Du general, $\frac{d}{d t} \int f(x, t) d x=\int \frac{\partial}{\partial t} f(x, t) d x$ if $f, \partial_{t} f$ are continuous and uniformly bounded, which means $|f(x, t)|<A(x),\left|\partial_{t} f(x, t)\right|<B(x)$ where $\int A(x) d x<\infty \int B(x) d x<\infty$.

$$
\begin{aligned}
\varphi^{\prime}(t) & =\sqrt{\frac{a}{2 \pi}} i \int d x \times e^{i x t} e^{-\frac{a}{2} x^{2}} \\
& =-\frac{i}{\sqrt{2 \pi a}} \int d x e^{i x t} \frac{d}{d x} e^{-\frac{a x^{2}}{2}} \quad \frac{d}{d x} e^{-\frac{a x^{2}}{2}}=-a x e^{-a x^{2}} \\
& =-\frac{t}{\sqrt{2 \pi a}} \int_{-\infty}^{+\infty} d x e^{i x t} e^{-\frac{a x^{2}}{2}} \\
& =-\frac{t}{a} \varphi(t)
\end{aligned}
$$

So $\quad \varphi^{\prime}=-\frac{t}{a} \varphi(t)$ and the solution is $\varphi(t)=c e^{-\frac{t^{2}}{2 a}}$ (check it out). However as $\varphi(0)=1 \Rightarrow c=1$,

$$
\begin{gathered}
\varphi(t)=e^{-\frac{t^{2}}{2 a}}=e^{\frac{b^{2}}{2 a}} \\
\hat{T}=i t
\end{gathered}
$$


\end{document}